% Set up the document
\documentclass{article}

% Page size
\usepackage[
    letterpaper,]{geometry}

% Lines between paragraphs
\setlength{\parskip}{\baselineskip}
\setlength{\parindent}{0pt}

% Math
\usepackage{amsmath}

% Links
\usepackage{hyperref}

\begin{document}

\section*{3. Social learning and replicator dynamics}

Here we have two behaviors: A and B. Without loss of generality, assume
behavior A has a higher payoff than behavior B. We're told that when a
two individuals meet, with one practicing behavior A and one practicing
behavior B, that each individual will adopt behavior A with probability
$1 - e$ and behaior B with probability $e$. When two individuals
practicing the same behavior meet, their behavior does not change. Hence

\begin{align*}
    P(A|A,A) &= 1 \\
    P(A|A,B) &= 1 - e \\
    P(A|B,A) &= 1 - e \\
    P(A|B,B) &= 0
\end{align*}

Letting $p$ be the probability that an individual in a population
practices behavior A, we have

\begin{align*}
    P(A,A) &= p^2 \\
    P(A,B) &= p(1 - p) \\
    P(B,A) &= p(1 - p) \\
    P(B,B) &= (1 - p)^2
\end{align*}

Hence the value of $p$ in the population's next generation, $p'$, is
given by

\begin{align*}
    p' &= P(A,A)P(A|A,A) + P(A,B)P(A|A,B) + P(B,A)P(A|B,A) + P(B,B)P(A|B,B) \\
       &= p^2 \cdot 1 + 2p(1 - p) \cdot (1 - e) + (1 - p)^2 \cdot 0 \\
       &= p^2 + 2p(1 - p)(1 - e) \\
       &= (2e - 1)p^2 + 2(1 - e)p
\end{align*}

and the change in frequency of A $\Delta p$ is given by

\begin{align*}
    \Delta p &= p' - p \\
             &= \{(2e - 1)p^2 + 2(1 - e)p\} - p \\
             &= (2e - 1)p^2 + (1 - 2e)p \\
             &= p(1 - p)(1 - 2e)
\end{align*}

\end{document}
